{
 "cells": [
  {
   "cell_type": "code",
   "execution_count": null,
   "id": "fe6d2977-c21d-4150-9fab-58d9b11a545e",
   "metadata": {},
   "outputs": [],
   "source": [
    "'''Q.1.). Find the val%e of T(2) for the rec%rrence relation T(n) = 3T(n-1) + 12n, given that T(0)=5.'''\n",
    "\n",
    "# Soolution :\n",
    "\n",
    "'''\n",
    "To find the value of T(2) for the given recurrence relation T(n) = 3T(n-1) + 12n with the initial condition T(0) = 5,\n",
    "we can use the recurrence relation iteratively.\n",
    "\n",
    "Given:\n",
    "T(0) = 5\n",
    "T(n) = 3T(n-1) + 12n \n",
    "\n",
    "Let's compute T(1) using the recurrence relation:\n",
    "\n",
    "T(1) = 3T(0) + 12 * 1 = 3 * 5 + 12 = 15 + 12 = 27\n",
    "\n",
    "Now, let's compute T(2) using the recurrence relation:\n",
    "\n",
    "T(2) = 3T(1) + 12 * 2 = 3 * 27 + 12 * 2 = 81 + 24 = 105\n",
    "\n",
    "So, the value of T(2) for the given recurrence relation with the initial condition T(0) = 5 is 105.\n",
    "'''"
   ]
  },
  {
   "cell_type": "code",
   "execution_count": null,
   "id": "0347e574-7623-4bde-bbc8-932ef3b2f567",
   "metadata": {},
   "outputs": [],
   "source": [
    "'''Q.2.). \n",
    "Given a recurrence relation, solve it using the substit%tion method:\n",
    "a. T(n) = T(n-1) + c\n",
    "b. T(n) = 2T(n/2) + n\n",
    "c. T(n) = 2T(n/2) + c\n",
    "d. T(n) = T(n/2) + c\n",
    "'''\n",
    "\n",
    "# Solution :\n",
    "\n",
    "'''\n",
    "To solve the given recurrence relations using the substitution method, we'll perform the following steps:\n",
    "\n",
    "1. Expand the recurrence relation recursively until we reach the base case or a known pattern.\n",
    "2. Make a guess for the form of the solution based on the observed pattern.\n",
    "3. Use mathematical induction to prove the correctness of our guess.\n",
    "\n",
    "Let's solve each recurrence relation:\n",
    "\n",
    "a. T(n) = T(n-1) + c\n",
    "\n",
    "This recurrence relation represents a linear increase. To solve it, we'll expand it:\n",
    "\n",
    "\n",
    "T(n) = T(n-1) + c\n",
    "     = T(n-2) + c + c\n",
    "     = T(n-3) + c + c + c\n",
    "     ...\n",
    "     = T(0) + nc\n",
    "\n",
    "Given the base case T(0), we can express the solution as:\n",
    "\n",
    "T(n) = T(0) + nc\n",
    "\n",
    "b. T(n) = 2T(n/2) + n\n",
    "\n",
    "This recurrence relation represents the divide-and-conquer paradigm, typical in algorithms like merge sort.\n",
    "To solve it, we'll make a guess that the solution is O(n log n). Let's prove it by substitution:\n",
    "\n",
    "Assume T(k) = O(k log k) for all k < n. Then:\n",
    "\n",
    "T(n) = 2T(n/2) + n <= 2(c(n/2 log(n/2))) + n\n",
    "     = cn log(n/2) + n\n",
    "     = cn(log n - log 2) + n\n",
    "     = cn log n - cn log 2 + n\n",
    "     = cn log n - cn + n\n",
    "\n",
    "Now, for n sufficiently large, n > cn, so:\n",
    "\n",
    "<= cn log n\n",
    "\n",
    "Thus, T(n) = O(n log n).\n",
    "\n",
    "c. T(n) = 2T(n/2) + c\n",
    "\n",
    "This recurrence relation is similar to the previous one but with a constant term instead of n.\n",
    "Using a similar approach as before, we can prove that T(n) = O(n).\n",
    "\n",
    "d. T(n) = T(n/2) + c\n",
    "\n",
    "This recurrence relation represents a linear increase. By expanding it, we can find:\n",
    "\n",
    "T(n) = T(n/2) + c = T(n/4) + c + c = T(n/8) + c + c + c = ...\n",
    "\n",
    "Continuing this pattern, we find:\n",
    "\n",
    "T(n) = T(1) + c log_2 n\n",
    "\n",
    "Since T(1) is a constant, T(n) = O(log n).\n",
    "\n",
    "These solutions provide an understanding of the growth rate of each recurrence relation with respect to the input size n.\n",
    "'''"
   ]
  },
  {
   "cell_type": "code",
   "execution_count": null,
   "id": "08694d6d-6747-4c52-a396-79dfc21148f2",
   "metadata": {},
   "outputs": [],
   "source": [
    "'''Q.3.). \n",
    "Given a recurrence relation, solve it using the recursive tree approach:\n",
    "a. T(n) = 2T(n-1) +1\n",
    "b. T(n) = 2T(n/2) + n\n",
    "'''\n",
    "\n",
    "# Solution :\n",
    "\n",
    "'''\n",
    "To solve the given recurrence relations using the recursive tree approach,\n",
    "we'll visualize the recursion tree and then analyze its structure to find a pattern or a closed-form solution.\n",
    "\n",
    "a. T(n) = 2T(n-1) + 1\n",
    "\n",
    "Let's construct the recursion tree for this recurrence relation:\n",
    "\n",
    "```\n",
    "                            T(n)\n",
    "                       /            \\\n",
    "                 T(n-1)            T(n-1)\n",
    "              /       \\          /       \\\n",
    "         T(n-2)      T(n-2)   T(n-2)   T(n-2)\n",
    "          / \\          / \\       / \\       / \\\n",
    "      T(n-3) T(n-3) T(n-3) T(n-3) T(n-3) T(n-3)\n",
    "        .      .      .      .      .      .\n",
    "        .      .      .      .      .      .\n",
    "```\n",
    "\n",
    "Each level of the tree has twice as many nodes as the previous level.\n",
    "At each level, we add 1 to the total cost. So, the total cost at level k is 2^k. The tree's height is n,\n",
    "so the total cost is:\n",
    "\n",
    "T(n) = 1 + 2 + 2^2 + ... + 2^n = 2^{n+1} - 1\n",
    "\n",
    "Therefore, T(n) = O(2^n).\n",
    "\n",
    "b. T(n) = 2T(n/2) + n\n",
    "\n",
    "Let's construct the recursion tree for this recurrence relation:\n",
    "\n",
    "```\n",
    "                            T(n)\n",
    "                       /            \\\n",
    "                 T(n/2)            T(n/2)\n",
    "              /       \\          /       \\\n",
    "          T(n/4)    T(n/4)   T(n/4)    T(n/4)\n",
    "           / \\        / \\       / \\        / \\\n",
    "       T(n/8) T(n/8) T(n/8) T(n/8) T(n/8) T(n/8)\n",
    "        .      .      .      .      .      .\n",
    "        .      .      .      .      .      .\n",
    "```\n",
    "\n",
    "At each level, the cost increases by n because each subproblem has size n/2 and we add n at the root.\n",
    "The tree's height is log n. So, the total cost is:\n",
    "\n",
    "T(n) = O(n log n)\n",
    "\n",
    "Therefore, T(n) = O(n log n).\n",
    "\n",
    "These solutions provide insights into the growth rate of each recurrence relation based on their respective recursion tree structures.\n",
    "'''"
   ]
  }
 ],
 "metadata": {
  "kernelspec": {
   "display_name": "Python 3 (ipykernel)",
   "language": "python",
   "name": "python3"
  },
  "language_info": {
   "codemirror_mode": {
    "name": "ipython",
    "version": 3
   },
   "file_extension": ".py",
   "mimetype": "text/x-python",
   "name": "python",
   "nbconvert_exporter": "python",
   "pygments_lexer": "ipython3",
   "version": "3.10.8"
  }
 },
 "nbformat": 4,
 "nbformat_minor": 5
}
